reorder

theories/crypto/oracle_PKE.ec
@@ -82,9 +82,10 @@ module Wrap (S : Scheme, LR : LR) : CCA_Oracle_i = {
   }
   
   proc l_or_r (m0 m1 : plaintext) : ciphertext = {
-    var c,m;
-    m <@ LR.l_or_r(m0,m1);
-    c <@ S.enc(pk,m);
+    var c, m;
+
+    m <@ LR.l_or_r(m0, m1);
+    c <@ S.enc(pk, m);
     cs <- c::cs;
     return c;
   }
@@ -94,24 +95,24 @@ module Wrap (S : Scheme, LR : LR) : CCA_Oracle_i = {
     
     m <- witness;
     if (! c \in cs) {
-      m <- S.dec(sk,c);
+      m <- S.dec(sk, c);
       ndec <- ndec + 1;
     }
     return m;
   }
 }.
 
-module CCA (S : Scheme, A:Adversary) = {
-
+module CCA (S : Scheme, A : Adversary) = {
   proc main() : bool = {
     var b';
+
     Wrap(S,LorR).init();
-    b' <@ A(Wrap(S,LorR)).main(Wrap.pk);
+    b' <@ A(Wrap(S, LorR)).main(Wrap.pk);
     return LorR.b = b';
   }
 }.
 
-module CCA_ (LR:LR, S : Scheme, A:Adversary) = {
+module CCA_ (S : Scheme, A : Adversary, LR : LR) = {
   proc main() : bool = {
     var b';
 
@@ -122,19 +123,19 @@ module CCA_ (LR:LR, S : Scheme, A:Adversary) = {
   }
 }.
 
-module CCA_L = CCA_(L).
-module CCA_R = CCA_(R).
+module CCA_L (S : Scheme, A : Adversary) = CCA_(S, A, L).
+module CCA_R (S : Scheme, A : Adversary) = CCA_(S, A, R).
 
 op Ndec : int.
 op Nenc : int.
 
-module B (A : Adversary, S : Scheme, O : CCA_Oracle) = {
+module B (S : Scheme, A : Adversary, O : CCA_Oracle) = {
   var i,iS : int
   var pk : pkey
   var cs : ciphertext list
   
   module O' : CCA_Oracle = {
-    proc l_or_r(m0,m1 : plaintext) = {
+    proc l_or_r(m0 m1 : plaintext) = {
       var c;
 
       if (i < iS) c <- S.enc(pk,m0);
@@ -149,6 +150,7 @@ module B (A : Adversary, S : Scheme, O : CCA_Oracle) = {
 
     proc dec(c:ciphertext) : plaintext option = {
       var m;
+
       m <- witness;
       if (! c \in cs) m <@ O.dec(c);
       return m;
@@ -169,8 +171,8 @@ module B (A : Adversary, S : Scheme, O : CCA_Oracle) = {
 
 section.
 
-declare module S : Scheme {Wrap,LorR,B}.
-declare module A : Adversary {Wrap, S, LorR,B}.
+declare module S : Scheme {Wrap, LorR, B}.
+declare module A : Adversary {Wrap, S, LorR, B}.
 
 axiom A_ll (O <: CCA_Oracle {A}) : 
   islossless O.l_or_r => islossless O.dec => islossless A(O).main.
@@ -181,16 +183,17 @@ axiom enc_ll : islossless S.enc.
 axiom dec_ll : islossless S.dec.
 
 lemma CCA_LR &m : 
-  `| Pr[ CCA(S,A).main() @ &m : res] - 1.0/2.0 | = 
-  1%r / 2%r * `| Pr[ CCA_L(S,A).main() @ &m : res ] - Pr[ CCA_R(S,A).main() @ &m : res ] |.
+  `| Pr[ CCA(S, A).main() @ &m : res] - 1.0/2.0 | = 
+  1%r / 2%r * `| Pr[ CCA_L(S, A).main() @ &m : res ] - Pr[ CCA_R(S, A).main() @ &m : res ] |.
 proof.
   rewrite (Top.LorR.pr_AdvLR_AdvRndLR (CCA_L(S,A)) (CCA_R(S,A)) &m).
     byphoare => //. 
-    islossless. apply: (A_ll(Wrap(S, R))). islossless. apply: enc_ll. 
-    islossless. apply: dec_ll. apply: kg_ll.
+    islossless; last by apply: kg_ll.
+    apply: (A_ll(Wrap(S, R))); first by islossless; apply: enc_ll. 
+    islossless; apply: dec_ll.
   suff <- : Pr[CCA(S, A).main() @ &m : res] = 
             Pr[Top.LorR.RandomLR(CCA_L(S,A),CCA_R(S,A)).main() @ &m : res] by smt().
-  byequiv => //; proc; inline *.
+  byequiv=> //. proc; inline *.
   seq 1 1 : (={glob A,glob S} /\ LorR.b{1} = b{2}); first by rnd.
   if{2}; wp. 
   - call (_ : ={glob S,glob Wrap} /\ LorR.b{1}).
@@ -206,7 +209,7 @@ proof.
 qed.
 
 axiom A_bound (O <: LR {Wrap, S, A}): 
-  hoare[ A(Wrap(S,O)).main : 
+  hoare[ A(Wrap(S, O)).main : 
     Wrap.ndec = 0 /\ Wrap.cs = [] ==> Wrap.ndec <= Ndec /\ size Wrap.cs <= Nenc].
 
 local module LRB (O : LR) : LR = {
@@ -214,7 +217,7 @@ local module LRB (O : LR) : LR = {
   
   proc init = O.init
 
-  proc l_or_r(m0,m1 : plaintext) = {
+  proc l_or_r(m0 m1 : plaintext) = {
     var m;
 
     if (i < iS) m <- m0;
@@ -228,50 +231,57 @@ local module LRB (O : LR) : LR = {
 }.
 
 local equiv eqv_WrapLRB (O <: LR {Wrap, S, A, B}) : 
-  A(B(A, S, Wrap(S, O)).O').main ~ A(Wrap(S,LRB(O))).main : 
-  ={glob A,glob Wrap,glob S, glob O, glob B} /\ ={pk} /\ Wrap.pk{1} = B.pk{1} /\
-   B.cs{1} = Wrap.cs{2} /\ (forall c, c \in Wrap.cs{1} => c \in Wrap.cs{2}) ==> ={Wrap.ndec}.
+  A(B(S, A, Wrap(S, O)).O').main ~ A(Wrap(S, LRB(O))).main : 
+  ={glob Wrap, glob O, glob S, glob A, glob B} /\ ={pk} /\
+  Wrap.pk{1} = B.pk{1} /\ B.cs{1} = Wrap.cs{2} /\
+  (forall c, c \in Wrap.cs{1} => c \in Wrap.cs{2}) ==> ={Wrap.ndec}.
 proof.
-  proc (={glob S, glob O} /\ ={Wrap.ndec, Wrap.sk, Wrap.pk, B.iS, B.i, B.pk} /\ 
-         B.cs{1} = Wrap.cs{2} /\ (forall c, c \in Wrap.cs{1} => c \in Wrap.cs{2}) /\
-         Wrap.pk{1} = B.pk{1}) => //.
-  + proc; inline *; sp.
-    if => //.
-    + by wp; call (:true); auto => /> /#.
-    if => //.
-    + by do 2!(wp; call (:true)); auto => /> /#.
+  proc (={glob O, glob S} /\ ={Wrap.ndec, Wrap.sk, Wrap.pk, B.iS, B.i, B.pk} /\ 
+        B.cs{1} = Wrap.cs{2} /\ (forall c, c \in Wrap.cs{1} => c \in Wrap.cs{2}) /\
+        Wrap.pk{1} = B.pk{1}) => //.
+  - proc; inline *; sp.
+    if => //; first by wp; call (:true); auto => /> /#.
+    if => //; first by do 2!(wp; call (:true)); auto => /> /#.
     by wp; call (:true); auto => /> /#.
-  proc. sp; if => //.
+  - proc; sp; if => //.
   inline *; rcondt{1} ^if; 1: by auto => /> /#.
   by wp; call(:true); auto.
 qed.
 
-lemma B_bound (O <: LR {Wrap, S, A,B}): 
-  hoare[ B(A,S,Wrap(S,O)).main : 
-    Wrap.ndec = 0 /\ Wrap.cs = [] /\ Wrap.pk = pk0 ==> Wrap.ndec <= Ndec /\ size Wrap.cs <= 1].
+lemma B_bound (O <: LR {Wrap, S, A, B}): 
+  hoare[B(S, A, Wrap(S,O)).main : 
+    Wrap.ndec = 0 /\ Wrap.cs = [] /\
+    Wrap.pk = pk0 ==> Wrap.ndec <= Ndec /\ size Wrap.cs <= 1].
 proof.
-  conseq (_ : Wrap.ndec = 0 /\ Wrap.cs = [] /\ Wrap.pk = pk0 ==> Wrap.ndec <= Ndec) 
-         (_ : Wrap.cs = [] ==> size Wrap.cs <= 1).
-  - done.
+  conseq (_ :
+    Wrap.ndec = 0 /\ Wrap.cs = [] /\ Wrap.pk = pk0
+    ==>
+    Wrap.ndec <= Ndec)
+         (_ : Wrap.cs = [] ==> size Wrap.cs <= 1) => //.
   - proc. 
     call (_ : size Wrap.cs = b2i (B.iS < B.i)).
-    + proc. inline *. 
+    + proc; inline *. 
       if; first by wp; call (:true); skip; smt().
       if; last by wp; call (: true); skip; smt().
       wp; sp; call (: true); call (: true); skip; smt().
     + by conseq />. 
-    + auto => />. smt(supp_dinter).
+    + auto => />; smt(supp_dinter).
   - proc.
-    call (_ : Wrap.ndec = 0 /\ Wrap.cs = [] /\ Wrap.pk = B.pk /\ B.cs = Wrap.cs ==> Wrap.ndec <= Ndec).
+    call (_ : Wrap.ndec = 0 /\ Wrap.cs = [] /\ Wrap.pk = B.pk /\
+              B.cs = Wrap.cs ==> Wrap.ndec <= Ndec).
     conseq (eqv_WrapLRB(O)) (A_bound(<: LRB(O))) => />; 1: smt().
     by auto.
 qed.
 
 lemma CCA_1n &m :
-    `| Pr[ CCA_L(S,A).main() @ &m : res ] - Pr[ CCA_R(S,A).main() @ &m : res ] | <= 
-    Nenc%r * `| Pr[ CCA_L(S,B(A,S)).main() @ &m : res ] - Pr[ CCA_R(S,B(A,S)).main() @ &m : res ] |.
-
-
+    `| Pr[ CCA_L(S,A).main() @ &m : res ] -
+       Pr[ CCA_R(S,A).main() @ &m : res ] |
+    <= 
+    Nenc%r
+    *
+    `| Pr[ CCA_L(S,B(S, A)).main() @ &m : res ] -
+       Pr[ CCA_R(S,B(S, A)).main() @ &m : res ] |.
+proof.
 admitted.
 
 end section.
